changed constant names and notation to match HOL/Subst/*.thy, from which this theory is a clone.

src/HOL/ex/Unification.thy
@@ -29,7 +29,7 @@ subsection {* Basic definitions *}
 datatype 'a trm = 
   Var 'a 
   | Const 'a
-  | App "'a trm" "'a trm" (infix "\<cdot>" 60)
+  | Comb "'a trm" "'a trm" (infix "\<cdot>" 60)
 
 type_synonym 'a subst = "('a \<times> 'a trm) list"
 
@@ -42,38 +42,38 @@ where
 
 text {* Applying a substitution to a term: *}
 
-fun apply_subst :: "'a trm \<Rightarrow> 'a subst \<Rightarrow> 'a trm" (infixl "\<triangleleft>" 60)
+primrec subst :: "'a trm \<Rightarrow> 'a subst \<Rightarrow> 'a trm" (infixl "\<lhd>" 55)
 where
-  "(Var v) \<triangleleft> s = assoc v (Var v) s"
-| "(Const c) \<triangleleft> s = (Const c)"
-| "(M \<cdot> N) \<triangleleft> s = (M \<triangleleft> s) \<cdot> (N \<triangleleft> s)"
+  "(Var v) \<lhd> s = assoc v (Var v) s"
+| "(Const c) \<lhd> s = (Const c)"
+| "(M \<cdot> N) \<lhd> s = (M \<lhd> s) \<cdot> (N \<lhd> s)"
 
 text {* Composition of substitutions: *}
 
 fun
-  "compose" :: "'a subst \<Rightarrow> 'a subst \<Rightarrow> 'a subst" (infixl "\<bullet>" 80)
+  comp :: "'a subst \<Rightarrow> 'a subst \<Rightarrow> 'a subst" (infixl "\<lozenge>" 56)
 where
-  "[] \<bullet> bl = bl"
-| "((a,b) # al) \<bullet> bl = (a, b \<triangleleft> bl) # (al \<bullet> bl)"
+  "[] \<lozenge> bl = bl"
+| "((a,b) # al) \<lozenge> bl = (a, b \<lhd> bl) # (al \<lozenge> bl)"
 
 text {* Equivalence of substitutions: *}
 
-definition eqv (infix "=\<^sub>s" 50)
+definition subst_eq (infixr "\<doteq>" 52)
 where
-  "s1 =\<^sub>s s2 \<equiv> \<forall>t. t \<triangleleft> s1 = t \<triangleleft> s2" 
+  "s1 \<doteq> s2 \<equiv> \<forall>t. t \<lhd> s1 = t \<lhd> s2" 
 
 
 subsection {* Basic lemmas *}
 
-lemma apply_empty[simp]: "t \<triangleleft> [] = t"
+lemma apply_empty[simp]: "t \<lhd> [] = t"
 by (induct t) auto
 
-lemma compose_empty[simp]: "\<sigma> \<bullet> [] = \<sigma>"
+lemma compose_empty[simp]: "\<sigma> \<lozenge> [] = \<sigma>"
 by (induct \<sigma>) auto
 
-lemma apply_compose[simp]: "t \<triangleleft> (s1 \<bullet> s2) = t \<triangleleft> s1 \<triangleleft> s2"
+lemma apply_compose[simp]: "t \<lhd> (s1 \<lozenge> s2) = t \<lhd> s1 \<lhd> s2"
 proof (induct t)
-  case App thus ?case by simp
+  case Comb thus ?case by simp
 next 
   case Const thus ?case by simp
 next
@@ -85,39 +85,39 @@ next
   qed
 qed
 
-lemma eqv_refl[intro]: "s =\<^sub>s s"
-  by (auto simp:eqv_def)
+lemma eqv_refl[intro]: "s \<doteq> s"
+  by (auto simp:subst_eq_def)
 
-lemma eqv_trans[trans]: "\<lbrakk>s1 =\<^sub>s s2; s2 =\<^sub>s s3\<rbrakk> \<Longrightarrow> s1 =\<^sub>s s3"
-  by (auto simp:eqv_def)
+lemma eqv_trans[trans]: "\<lbrakk>s1 \<doteq> s2; s2 \<doteq> s3\<rbrakk> \<Longrightarrow> s1 \<doteq> s3"
+  by (auto simp:subst_eq_def)
 
-lemma eqv_sym[sym]: "\<lbrakk>s1 =\<^sub>s s2\<rbrakk> \<Longrightarrow> s2 =\<^sub>s s1"
-  by (auto simp:eqv_def)
+lemma eqv_sym[sym]: "\<lbrakk>s1 \<doteq> s2\<rbrakk> \<Longrightarrow> s2 \<doteq> s1"
+  by (auto simp:subst_eq_def)
 
-lemma eqv_intro[intro]: "(\<And>t. t \<triangleleft> \<sigma> = t \<triangleleft> \<theta>) \<Longrightarrow> \<sigma> =\<^sub>s \<theta>"
-  by (auto simp:eqv_def)
+lemma eqv_intro[intro]: "(\<And>t. t \<lhd> \<sigma> = t \<lhd> \<theta>) \<Longrightarrow> \<sigma> \<doteq> \<theta>"
+  by (auto simp:subst_eq_def)
 
-lemma eqv_dest[dest]: "s1 =\<^sub>s s2 \<Longrightarrow> t \<triangleleft> s1 = t \<triangleleft> s2"
-  by (auto simp:eqv_def)
+lemma eqv_dest[dest]: "s1 \<doteq> s2 \<Longrightarrow> t \<lhd> s1 = t \<lhd> s2"
+  by (auto simp:subst_eq_def)
 
-lemma compose_eqv: "\<lbrakk>\<sigma> =\<^sub>s \<sigma>'; \<theta> =\<^sub>s \<theta>'\<rbrakk> \<Longrightarrow> (\<sigma> \<bullet> \<theta>) =\<^sub>s (\<sigma>' \<bullet> \<theta>')"
-  by (auto simp:eqv_def)
+lemma compose_eqv: "\<lbrakk>\<sigma> \<doteq> \<sigma>'; \<theta> \<doteq> \<theta>'\<rbrakk> \<Longrightarrow> (\<sigma> \<lozenge> \<theta>) \<doteq> (\<sigma>' \<lozenge> \<theta>')"
+  by (auto simp:subst_eq_def)
 
-lemma compose_assoc: "(a \<bullet> b) \<bullet> c =\<^sub>s a \<bullet> (b \<bullet> c)"
+lemma compose_assoc: "(a \<lozenge> b) \<lozenge> c \<doteq> a \<lozenge> (b \<lozenge> c)"
   by auto
 
 
 subsection {* Specification: Most general unifiers *}
 
 definition
-  "Unifier \<sigma> t u \<equiv> (t\<triangleleft>\<sigma> = u\<triangleleft>\<sigma>)"
+  "Unifier \<sigma> t u \<equiv> (t\<lhd>\<sigma> = u\<lhd>\<sigma>)"
 
 definition
   "MGU \<sigma> t u \<equiv> Unifier \<sigma> t u \<and> (\<forall>\<theta>. Unifier \<theta> t u 
-  \<longrightarrow> (\<exists>\<gamma>. \<theta> =\<^sub>s \<sigma> \<bullet> \<gamma>))"
+  \<longrightarrow> (\<exists>\<gamma>. \<theta> \<doteq> \<sigma> \<lozenge> \<gamma>))"
 
 lemma MGUI[intro]:
-  "\<lbrakk>t \<triangleleft> \<sigma> = u \<triangleleft> \<sigma>; \<And>\<theta>. t \<triangleleft> \<theta> = u \<triangleleft> \<theta> \<Longrightarrow> \<exists>\<gamma>. \<theta> =\<^sub>s \<sigma> \<bullet> \<gamma>\<rbrakk>
+  "\<lbrakk>t \<lhd> \<sigma> = u \<lhd> \<sigma>; \<And>\<theta>. t \<lhd> \<theta> = u \<lhd> \<theta> \<Longrightarrow> \<exists>\<gamma>. \<theta> \<doteq> \<sigma> \<lozenge> \<gamma>\<rbrakk>
   \<Longrightarrow> MGU \<sigma> t u"
   by (simp only:Unifier_def MGU_def, auto)
 
@@ -130,11 +130,11 @@ subsection {* The unification algorithm *}
 
 text {* Occurs check: Proper subterm relation *}
 
-fun occ :: "'a trm \<Rightarrow> 'a trm \<Rightarrow> bool"
+fun occs :: "'a trm \<Rightarrow> 'a trm \<Rightarrow> bool" (infixl "<:" 54) 
 where
-  "occ u (Var v) = False"
-| "occ u (Const c) = False"
-| "occ u (M \<cdot> N) = (u = M \<or> u = N \<or> occ u M \<or> occ u N)"
+  "occs u (Var v) = False"
+| "occs u (Const c) = False"
+| "occs u (M \<cdot> N) = (u = M \<or> u = N \<or> occs u M \<or> occs u N)"
 
 text {* The unification algorithm: *}
 
@@ -143,41 +143,41 @@ where
   "unify (Const c) (M \<cdot> N)   = None"
 | "unify (M \<cdot> N)   (Const c) = None"
 | "unify (Const c) (Var v)   = Some [(v, Const c)]"
-| "unify (M \<cdot> N)   (Var v)   = (if (occ (Var v) (M \<cdot> N)) 
+| "unify (M \<cdot> N)   (Var v)   = (if (occs (Var v) (M \<cdot> N)) 
                                         then None
                                         else Some [(v, M \<cdot> N)])"
-| "unify (Var v)   M         = (if (occ (Var v) M) 
+| "unify (Var v)   M         = (if (occs (Var v) M) 
                                         then None
                                         else Some [(v, M)])"
 | "unify (Const c) (Const d) = (if c=d then Some [] else None)"
 | "unify (M \<cdot> N) (M' \<cdot> N') = (case unify M M' of
                                     None \<Rightarrow> None |
-                                    Some \<theta> \<Rightarrow> (case unify (N \<triangleleft> \<theta>) (N' \<triangleleft> \<theta>)
+                                    Some \<theta> \<Rightarrow> (case unify (N \<lhd> \<theta>) (N' \<lhd> \<theta>)
                                       of None \<Rightarrow> None |
-                                         Some \<sigma> \<Rightarrow> Some (\<theta> \<bullet> \<sigma>)))"
+                                         Some \<sigma> \<Rightarrow> Some (\<theta> \<lozenge> \<sigma>)))"
   by pat_completeness auto
 
 declare unify.psimps[simp]
 
 subsection {* Partial correctness *}
 
-text {* Some lemmas about occ and MGU: *}
+text {* Some lemmas about occs and MGU: *}
 
-lemma subst_no_occ: "\<not>occ (Var v) t \<Longrightarrow> Var v \<noteq> t
-  \<Longrightarrow> t \<triangleleft> [(v,s)] = t"
+lemma subst_no_occs: "\<not>occs (Var v) t \<Longrightarrow> Var v \<noteq> t
+  \<Longrightarrow> t \<lhd> [(v,s)] = t"
 by (induct t) auto
 
 lemma MGU_Var[intro]: 
-  assumes no_occ: "\<not>occ (Var v) t"
+  assumes no_occs: "\<not>occs (Var v) t"
   shows "MGU [(v,t)] (Var v) t"
 proof (intro MGUI exI)
-  show "Var v \<triangleleft> [(v,t)] = t \<triangleleft> [(v,t)]" using no_occ
-    by (cases "Var v = t", auto simp:subst_no_occ)
+  show "Var v \<lhd> [(v,t)] = t \<lhd> [(v,t)]" using no_occs
+    by (cases "Var v = t", auto simp:subst_no_occs)
 next
-  fix \<theta> assume th: "Var v \<triangleleft> \<theta> = t \<triangleleft> \<theta>" 
-  show "\<theta> =\<^sub>s [(v,t)] \<bullet> \<theta>" 
+  fix \<theta> assume th: "Var v \<lhd> \<theta> = t \<lhd> \<theta>" 
+  show "\<theta> \<doteq> [(v,t)] \<lozenge> \<theta>" 
   proof
-    fix s show "s \<triangleleft> \<theta> = s \<triangleleft> [(v,t)] \<bullet> \<theta>" using th 
+    fix s show "s \<lhd> \<theta> = s \<lhd> [(v,t)] \<lozenge> \<theta>" using th 
       by (induct s) auto
   qed
 qed
@@ -200,42 +200,42 @@ proof (induct M N arbitrary: \<sigma>)
 
   then obtain \<theta>1 \<theta>2 
     where "unify M M' = Some \<theta>1"
-    and "unify (N \<triangleleft> \<theta>1) (N' \<triangleleft> \<theta>1) = Some \<theta>2"
-    and \<sigma>: "\<sigma> = \<theta>1 \<bullet> \<theta>2"
+    and "unify (N \<lhd> \<theta>1) (N' \<lhd> \<theta>1) = Some \<theta>2"
+    and \<sigma>: "\<sigma> = \<theta>1 \<lozenge> \<theta>2"
     and MGU_inner: "MGU \<theta>1 M M'" 
-    and MGU_outer: "MGU \<theta>2 (N \<triangleleft> \<theta>1) (N' \<triangleleft> \<theta>1)"
+    and MGU_outer: "MGU \<theta>2 (N \<lhd> \<theta>1) (N' \<lhd> \<theta>1)"
     by (auto split:option.split_asm)
 
   show ?case
   proof
     from MGU_inner and MGU_outer
-    have "M \<triangleleft> \<theta>1 = M' \<triangleleft> \<theta>1" 
-      and "N \<triangleleft> \<theta>1 \<triangleleft> \<theta>2 = N' \<triangleleft> \<theta>1 \<triangleleft> \<theta>2"
+    have "M \<lhd> \<theta>1 = M' \<lhd> \<theta>1" 
+      and "N \<lhd> \<theta>1 \<lhd> \<theta>2 = N' \<lhd> \<theta>1 \<lhd> \<theta>2"
       unfolding MGU_def Unifier_def
       by auto
-    thus "M \<cdot> N \<triangleleft> \<sigma> = M' \<cdot> N' \<triangleleft> \<sigma>" unfolding \<sigma>
+    thus "M \<cdot> N \<lhd> \<sigma> = M' \<cdot> N' \<lhd> \<sigma>" unfolding \<sigma>
       by simp
   next
-    fix \<sigma>' assume "M \<cdot> N \<triangleleft> \<sigma>' = M' \<cdot> N' \<triangleleft> \<sigma>'"
-    hence "M \<triangleleft> \<sigma>' = M' \<triangleleft> \<sigma>'"
-      and Ns: "N \<triangleleft> \<sigma>' = N' \<triangleleft> \<sigma>'" by auto
+    fix \<sigma>' assume "M \<cdot> N \<lhd> \<sigma>' = M' \<cdot> N' \<lhd> \<sigma>'"
+    hence "M \<lhd> \<sigma>' = M' \<lhd> \<sigma>'"
+      and Ns: "N \<lhd> \<sigma>' = N' \<lhd> \<sigma>'" by auto
 
     with MGU_inner obtain \<delta>
-      where eqv: "\<sigma>' =\<^sub>s \<theta>1 \<bullet> \<delta>"
+      where eqv: "\<sigma>' \<doteq> \<theta>1 \<lozenge> \<delta>"
       unfolding MGU_def Unifier_def
       by auto
 
-    from Ns have "N \<triangleleft> \<theta>1 \<triangleleft> \<delta> = N' \<triangleleft> \<theta>1 \<triangleleft> \<delta>"
+    from Ns have "N \<lhd> \<theta>1 \<lhd> \<delta> = N' \<lhd> \<theta>1 \<lhd> \<delta>"
       by (simp add:eqv_dest[OF eqv])
 
     with MGU_outer obtain \<rho>
-      where eqv2: "\<delta> =\<^sub>s \<theta>2 \<bullet> \<rho>"
+      where eqv2: "\<delta> \<doteq> \<theta>2 \<lozenge> \<rho>"
       unfolding MGU_def Unifier_def
       by auto
     
-    have "\<sigma>' =\<^sub>s \<sigma> \<bullet> \<rho>" unfolding \<sigma>
+    have "\<sigma>' \<doteq> \<sigma> \<lozenge> \<rho>" unfolding \<sigma>
       by (rule eqv_intro, auto simp:eqv_dest[OF eqv] eqv_dest[OF eqv2])
-    thus "\<exists>\<gamma>. \<sigma>' =\<^sub>s \<sigma> \<bullet> \<gamma>" ..
+    thus "\<exists>\<gamma>. \<sigma>' \<doteq> \<sigma> \<lozenge> \<gamma>" ..
   qed
 qed (auto split:split_if_asm) -- "Solve the remaining cases automatically"
 
@@ -256,50 +256,50 @@ lemma vars_of_finite[intro]: "finite (vars_of t)"
 text {* Elimination of variables by a substitution: *}
 
 definition
-  "elim \<sigma> v \<equiv> \<forall>t. v \<notin> vars_of (t \<triangleleft> \<sigma>)"
+  "elim \<sigma> v \<equiv> \<forall>t. v \<notin> vars_of (t \<lhd> \<sigma>)"
 
-lemma elim_intro[intro]: "(\<And>t. v \<notin> vars_of (t \<triangleleft> \<sigma>)) \<Longrightarrow> elim \<sigma> v"
+lemma elim_intro[intro]: "(\<And>t. v \<notin> vars_of (t \<lhd> \<sigma>)) \<Longrightarrow> elim \<sigma> v"
   by (auto simp:elim_def)
 
-lemma elim_dest[dest]: "elim \<sigma> v \<Longrightarrow> v \<notin> vars_of (t \<triangleleft> \<sigma>)"
+lemma elim_dest[dest]: "elim \<sigma> v \<Longrightarrow> v \<notin> vars_of (t \<lhd> \<sigma>)"
   by (auto simp:elim_def)
 
-lemma elim_eqv: "\<sigma> =\<^sub>s \<theta> \<Longrightarrow> elim \<sigma> x = elim \<theta> x"
-  by (auto simp:elim_def eqv_def)
+lemma elim_eqv: "\<sigma> \<doteq> \<theta> \<Longrightarrow> elim \<sigma> x = elim \<theta> x"
+  by (auto simp:elim_def subst_eq_def)
 
 
 text {* Replacing a variable by itself yields an identity subtitution: *}
 
-lemma var_self[intro]: "[(v, Var v)] =\<^sub>s []"
+lemma var_self[intro]: "[(v, Var v)] \<doteq> []"
 proof
-  fix t show "t \<triangleleft> [(v, Var v)] = t \<triangleleft> []"
+  fix t show "t \<lhd> [(v, Var v)] = t \<lhd> []"
     by (induct t) simp_all
 qed
 
-lemma var_same: "([(v, t)] =\<^sub>s []) = (t = Var v)"
+lemma var_same: "([(v, t)] \<doteq> []) = (t = Var v)"
 proof
   assume t_v: "t = Var v"
-  thus "[(v, t)] =\<^sub>s []"
+  thus "[(v, t)] \<doteq> []"
     by auto
 next
-  assume id: "[(v, t)] =\<^sub>s []"
+  assume id: "[(v, t)] \<doteq> []"
   show "t = Var v"
   proof -
-    have "t = Var v \<triangleleft> [(v, t)]" by simp
-    also from id have "\<dots> = Var v \<triangleleft> []" ..
+    have "t = Var v \<lhd> [(v, t)]" by simp
+    also from id have "\<dots> = Var v \<lhd> []" ..
     finally show ?thesis by simp
   qed
 qed
 
-text {* A lemma about occ and elim *}
+text {* A lemma about occs and elim *}
 
 lemma remove_var:
   assumes [simp]: "v \<notin> vars_of s"
-  shows "v \<notin> vars_of (t \<triangleleft> [(v, s)])"
+  shows "v \<notin> vars_of (t \<lhd> [(v, s)])"
   by (induct t) simp_all
 
-lemma occ_elim: "\<not>occ (Var v) t 
-  \<Longrightarrow> elim [(v,t)] v \<or> [(v,t)] =\<^sub>s []"
+lemma occs_elim: "\<not>occs (Var v) t 
+  \<Longrightarrow> elim [(v,t)] v \<or> [(v,t)] \<doteq> []"
 proof (induct t)
   case (Var x)
   show ?case
@@ -319,29 +319,29 @@ next
     by (auto intro!:remove_var)
   thus ?case ..
 next
-  case (App M N)
+  case (Comb M N)
   
-  hence ih1: "elim [(v, M)] v \<or> [(v, M)] =\<^sub>s []"
-    and ih2: "elim [(v, N)] v \<or> [(v, N)] =\<^sub>s []"
-    and nonocc: "Var v \<noteq> M" "Var v \<noteq> N"
+  hence ih1: "elim [(v, M)] v \<or> [(v, M)] \<doteq> []"
+    and ih2: "elim [(v, N)] v \<or> [(v, N)] \<doteq> []"
+    and nonoccs: "Var v \<noteq> M" "Var v \<noteq> N"
     by auto
 
-  from nonocc have "\<not> [(v,M)] =\<^sub>s []"
+  from nonoccs have "\<not> [(v,M)] \<doteq> []"
     by (simp add:var_same)
   with ih1 have "elim [(v, M)] v" by blast
-  hence "v \<notin> vars_of (Var v \<triangleleft> [(v,M)])" ..
+  hence "v \<notin> vars_of (Var v \<lhd> [(v,M)])" ..
   hence not_in_M: "v \<notin> vars_of M" by simp
 
-  from nonocc have "\<not> [(v,N)] =\<^sub>s []"
+  from nonoccs have "\<not> [(v,N)] \<doteq> []"
     by (simp add:var_same)
   with ih2 have "elim [(v, N)] v" by blast
-  hence "v \<notin> vars_of (Var v \<triangleleft> [(v,N)])" ..
+  hence "v \<notin> vars_of (Var v \<lhd> [(v,N)])" ..
   hence not_in_N: "v \<notin> vars_of N" by simp
 
   have "elim [(v, M \<cdot> N)] v"
   proof 
     fix t 
-    show "v \<notin> vars_of (t \<triangleleft> [(v, M \<cdot> N)])"
+    show "v \<notin> vars_of (t \<lhd> [(v, M \<cdot> N)])"
     proof (induct t)
       case (Var x) thus ?case by (simp add: not_in_M not_in_N)
     qed auto
@@ -354,7 +354,7 @@ text {* The result of a unification never introduces new variables: *}
 lemma unify_vars: 
   assumes "unify_dom (M, N)"
   assumes "unify M N = Some \<sigma>"
-  shows "vars_of (t \<triangleleft> \<sigma>) \<subseteq> vars_of M \<union> vars_of N \<union> vars_of t"
+  shows "vars_of (t \<lhd> \<sigma>) \<subseteq> vars_of M \<union> vars_of N \<union> vars_of t"
   (is "?P M N \<sigma> t")
 using assms
 proof (induct M N arbitrary:\<sigma> t)
@@ -363,45 +363,45 @@ proof (induct M N arbitrary:\<sigma> t)
   thus ?case by (induct t) auto
 next
   case (4 M N v) 
-  hence "\<not>occ (Var v) (M\<cdot>N)" by (cases "occ (Var v) (M\<cdot>N)", auto)
+  hence "\<not>occs (Var v) (M\<cdot>N)" by (cases "occs (Var v) (M\<cdot>N)", auto)
   with 4 have "\<sigma> = [(v, M\<cdot>N)]" by simp
   thus ?case by (induct t) auto
 next
   case (5 v M)
-  hence "\<not>occ (Var v) M" by (cases "occ (Var v) M", auto)
+  hence "\<not>occs (Var v) M" by (cases "occs (Var v) M", auto)
   with 5 have "\<sigma> = [(v, M)]" by simp
   thus ?case by (induct t) auto
 next
   case (7 M N M' N' \<sigma>)
   then obtain \<theta>1 \<theta>2 
     where "unify M M' = Some \<theta>1"
-    and "unify (N \<triangleleft> \<theta>1) (N' \<triangleleft> \<theta>1) = Some \<theta>2"
-    and \<sigma>: "\<sigma> = \<theta>1 \<bullet> \<theta>2"
+    and "unify (N \<lhd> \<theta>1) (N' \<lhd> \<theta>1) = Some \<theta>2"
+    and \<sigma>: "\<sigma> = \<theta>1 \<lozenge> \<theta>2"
     and ih1: "\<And>t. ?P M M' \<theta>1 t"
-    and ih2: "\<And>t. ?P (N\<triangleleft>\<theta>1) (N'\<triangleleft>\<theta>1) \<theta>2 t"
+    and ih2: "\<And>t. ?P (N\<lhd>\<theta>1) (N'\<lhd>\<theta>1) \<theta>2 t"
     by (auto split:option.split_asm)
 
   show ?case
   proof
-    fix v assume a: "v \<in> vars_of (t \<triangleleft> \<sigma>)"
+    fix v assume a: "v \<in> vars_of (t \<lhd> \<sigma>)"
     
     show "v \<in> vars_of (M \<cdot> N) \<union> vars_of (M' \<cdot> N') \<union> vars_of t"
     proof (cases "v \<notin> vars_of M \<and> v \<notin> vars_of M'
         \<and> v \<notin> vars_of N \<and> v \<notin> vars_of N'")
       case True
-      with ih1 have l:"\<And>t. v \<in> vars_of (t \<triangleleft> \<theta>1) \<Longrightarrow> v \<in> vars_of t"
+      with ih1 have l:"\<And>t. v \<in> vars_of (t \<lhd> \<theta>1) \<Longrightarrow> v \<in> vars_of t"
         by auto
       
-      from a and ih2[where t="t \<triangleleft> \<theta>1"]
-      have "v \<in> vars_of (N \<triangleleft> \<theta>1) \<union> vars_of (N' \<triangleleft> \<theta>1) 
-        \<or> v \<in> vars_of (t \<triangleleft> \<theta>1)" unfolding \<sigma>
+      from a and ih2[where t="t \<lhd> \<theta>1"]
+      have "v \<in> vars_of (N \<lhd> \<theta>1) \<union> vars_of (N' \<lhd> \<theta>1) 
+        \<or> v \<in> vars_of (t \<lhd> \<theta>1)" unfolding \<sigma>
         by auto
       hence "v \<in> vars_of t"
       proof
-        assume "v \<in> vars_of (N \<triangleleft> \<theta>1) \<union> vars_of (N' \<triangleleft> \<theta>1)"
+        assume "v \<in> vars_of (N \<lhd> \<theta>1) \<union> vars_of (N' \<lhd> \<theta>1)"
         with True show ?thesis by (auto dest:l)
       next
-        assume "v \<in> vars_of (t \<triangleleft> \<theta>1)" 
+        assume "v \<in> vars_of (t \<lhd> \<theta>1)" 
         thus ?thesis by (rule l)
       qed
       
@@ -417,7 +417,7 @@ substitution or it eliminates a variable from one of the terms: *}
 lemma unify_eliminates: 
   assumes "unify_dom (M, N)"
   assumes "unify M N = Some \<sigma>"
-  shows "(\<exists>v\<in>vars_of M \<union> vars_of N. elim \<sigma> v) \<or> \<sigma> =\<^sub>s []"
+  shows "(\<exists>v\<in>vars_of M \<union> vars_of N. elim \<sigma> v) \<or> \<sigma> \<doteq> []"
   (is "?P M N \<sigma>")
 using assms
 proof (induct M N arbitrary:\<sigma>)
@@ -426,21 +426,21 @@ next
   case 2 thus ?case by simp
 next
   case (3 c v)
-  have no_occ: "\<not> occ (Var v) (Const c)" by simp
+  have no_occs: "\<not> occs (Var v) (Const c)" by simp
   with 3 have "\<sigma> = [(v, Const c)]" by simp
-  with occ_elim[OF no_occ]
+  with occs_elim[OF no_occs]
   show ?case by auto
 next
   case (4 M N v)
-  hence no_occ: "\<not>occ (Var v) (M\<cdot>N)" by (cases "occ (Var v) (M\<cdot>N)", auto)
+  hence no_occs: "\<not>occs (Var v) (M\<cdot>N)" by (cases "occs (Var v) (M\<cdot>N)", auto)
   with 4 have "\<sigma> = [(v, M\<cdot>N)]" by simp
-  with occ_elim[OF no_occ]
+  with occs_elim[OF no_occs]
   show ?case by auto 
 next
   case (5 v M) 
-  hence no_occ: "\<not>occ (Var v) M" by (cases "occ (Var v) M", auto)
+  hence no_occs: "\<not>occs (Var v) M" by (cases "occs (Var v) M", auto)
   with 5 have "\<sigma> = [(v, M)]" by simp
-  with occ_elim[OF no_occ]
+  with occs_elim[OF no_occs]
   show ?case by auto 
 next 
   case (6 c d) thus ?case
@@ -449,43 +449,43 @@ next
   case (7 M N M' N' \<sigma>)
   then obtain \<theta>1 \<theta>2 
     where "unify M M' = Some \<theta>1"
-    and "unify (N \<triangleleft> \<theta>1) (N' \<triangleleft> \<theta>1) = Some \<theta>2"
-    and \<sigma>: "\<sigma> = \<theta>1 \<bullet> \<theta>2"
+    and "unify (N \<lhd> \<theta>1) (N' \<lhd> \<theta>1) = Some \<theta>2"
+    and \<sigma>: "\<sigma> = \<theta>1 \<lozenge> \<theta>2"
     and ih1: "?P M M' \<theta>1"
-    and ih2: "?P (N\<triangleleft>\<theta>1) (N'\<triangleleft>\<theta>1) \<theta>2"
+    and ih2: "?P (N\<lhd>\<theta>1) (N'\<lhd>\<theta>1) \<theta>2"
     by (auto split:option.split_asm)
 
   from `unify_dom (M \<cdot> N, M' \<cdot> N')`
   have "unify_dom (M, M')"
     by (rule accp_downward) (rule unify_rel.intros)
   hence no_new_vars: 
-    "\<And>t. vars_of (t \<triangleleft> \<theta>1) \<subseteq> vars_of M \<union> vars_of M' \<union> vars_of t"
+    "\<And>t. vars_of (t \<lhd> \<theta>1) \<subseteq> vars_of M \<union> vars_of M' \<union> vars_of t"
     by (rule unify_vars) (rule `unify M M' = Some \<theta>1`)
 
   from ih2 show ?case 
   proof 
-    assume "\<exists>v\<in>vars_of (N \<triangleleft> \<theta>1) \<union> vars_of (N' \<triangleleft> \<theta>1). elim \<theta>2 v"
+    assume "\<exists>v\<in>vars_of (N \<lhd> \<theta>1) \<union> vars_of (N' \<lhd> \<theta>1). elim \<theta>2 v"
     then obtain v 
-      where "v\<in>vars_of (N \<triangleleft> \<theta>1) \<union> vars_of (N' \<triangleleft> \<theta>1)"
+      where "v\<in>vars_of (N \<lhd> \<theta>1) \<union> vars_of (N' \<lhd> \<theta>1)"
       and el: "elim \<theta>2 v" by auto
     with no_new_vars show ?thesis unfolding \<sigma> 
       by (auto simp:elim_def)
   next
-    assume empty[simp]: "\<theta>2 =\<^sub>s []"
+    assume empty[simp]: "\<theta>2 \<doteq> []"
 
-    have "\<sigma> =\<^sub>s (\<theta>1 \<bullet> [])" unfolding \<sigma>
+    have "\<sigma> \<doteq> (\<theta>1 \<lozenge> [])" unfolding \<sigma>
       by (rule compose_eqv) auto
-    also have "\<dots> =\<^sub>s \<theta>1" by auto
-    finally have "\<sigma> =\<^sub>s \<theta>1" .
+    also have "\<dots> \<doteq> \<theta>1" by auto
+    finally have "\<sigma> \<doteq> \<theta>1" .
 
     from ih1 show ?thesis
     proof
       assume "\<exists>v\<in>vars_of M \<union> vars_of M'. elim \<theta>1 v"
-      with elim_eqv[OF `\<sigma> =\<^sub>s \<theta>1`]
+      with elim_eqv[OF `\<sigma> \<doteq> \<theta>1`]
       show ?thesis by auto
     next
-      note `\<sigma> =\<^sub>s \<theta>1`
-      also assume "\<theta>1 =\<^sub>s []"
+      note `\<sigma> \<doteq> \<theta>1`
+      also assume "\<theta>1 \<doteq> []"
       finally show ?thesis ..
     qed
   qed
@@ -509,7 +509,7 @@ proof
     "unify M M' = Some \<theta>"
 
   from unify_eliminates[OF inner]
-  show "((N \<triangleleft> \<theta>, N' \<triangleleft> \<theta>), (M \<cdot> N, M' \<cdot> N')) \<in>?R"
+  show "((N \<lhd> \<theta>, N' \<lhd> \<theta>), (M \<cdot> N, M' \<cdot> N')) \<in>?R"
   proof
     -- {* Either a variable is eliminated \ldots *}
     assume "(\<exists>v\<in>vars_of M \<union> vars_of M'. elim \<theta> v)"
@@ -517,7 +517,7 @@ proof
       where "elim \<theta> v" 
       and "v\<in>vars_of M \<union> vars_of M'" by auto
     with unify_vars[OF inner]
-    have "vars_of (N\<triangleleft>\<theta>) \<union> vars_of (N'\<triangleleft>\<theta>)
+    have "vars_of (N\<lhd>\<theta>) \<union> vars_of (N'\<lhd>\<theta>)
       \<subset> vars_of (M\<cdot>N) \<union> vars_of (M'\<cdot>N')"
       by auto
     
@@ -525,9 +525,9 @@ proof
       by (auto intro!: measures_less intro: psubset_card_mono)
   next
     -- {* Or the substitution is empty *}
-    assume "\<theta> =\<^sub>s []"
-    hence "N \<triangleleft> \<theta> = N" 
-      and "N' \<triangleleft> \<theta> = N'" by auto
+    assume "\<theta> \<doteq> []"
+    hence "N \<lhd> \<theta> = N" 
+      and "N' \<lhd> \<theta> = N'" by auto
     thus ?thesis 
        by (auto intro!: measures_less intro: psubset_card_mono)
   qed
